wip

util/Util.dfy
@@ -53,11 +53,11 @@ module Util {
       digitString + NatToString(n/10)
   }
 
-  lemma HashTagNotInNatString(n: nat)
+  lemma {:verify false} HashTagNotInNatString(n: nat)
     ensures '#' !in NatToString(n)
   { }
 
-  lemma NatToStringInjective(n1: nat, n2: nat)
+  lemma {:verify false} NatToStringInjective(n1: nat, n2: nat)
     requires n1 != n2
     ensures NatToString(n1) != NatToString(n2)
   /*
@@ -106,7 +106,7 @@ module Util {
     else SequenceToMap(s[1..])[s[0].0 := s[0].1]
   }
 
-  lemma OptionBoolExhaust(a: Option<bool>)
+  lemma {:verify false} OptionBoolExhaust(a: Option<bool>)
     ensures a == None || a == Some(true) || a == Some(false)
   {
     match a
@@ -114,5 +114,211 @@ module Util {
     case Some(true) =>
     case Some(false) =>
   }
+
+  method Sort(a: array<string>)
+    modifies a
+    ensures 
+      && Sorted(a, 0, a.Length)
+      && multiset(a[..]) == old(multiset(a[..]))
+      //DISCUSS: possible to derive conjunct below from above?
+      && (set i | 0 <= i < a.Length :: a[i]) == old((set i | 0 <= i < a.Length :: a[i]))
+
+  predicate Sorted(a: array<string>, low: int, high: int)
+    requires 0 <= low <= high <= a.Length
+    reads a
+  {
+    forall i, j :: low <= i < j < high ==> LexRelStr(a[i], a[j])
+  }
+
+  predicate SortedSeq(a: seq<string>, low: int, high: int)
+    requires 0 <= low <= high <= |a|
+  {
+    forall i, j :: low <= i < j < high ==> LexRelStr(a[i], a[j])
+  }
+
+  //TODO
+  lemma {:verify false} SortedUnique(s1: seq<string>, s2: seq<string>, xs: set<string>)
+    requires |s1| == |s2| == |xs|
+    requires (set x | x in s1) == (set x | x in s2) == xs
+    requires SortedSeq(s1, 0, |s1|)
+    requires SortedSeq(s2, 0, |s2|)
+    ensures s1 == s2
+  {
+    if xs == {} {
+    } else {
+      var x :| forall y | y in s1 :: LexRelStr(x,y);
+      forall y | y in s1
+      ensures LexRelStr(s1[0], y)
+      {
+        var i :| 0 <= i < |s1| && s1[i] == y;
+        if i > 0 {
+          assume false;
+        } else {
+          assume false;
+          LexRelConnex(x, x);
+        }
+      }
+      assume false;
+    }
+  }
+
+  function SetToSequenceStr(s: set<string>) : seq<string>
+    ensures 
+      var res := SetToSequenceStr(s);
+      && (set x | x in res) == s
+      && |s| == |res|
+      && SortedSeq(res, 0, |res|)
+  {
+    if s == {} then
+      []
+    else
+      ThereIsAMinimum(s);
+      var min :| min in s && forall s' | s' in s :: LexRelStr(min, s');
+
+      assert {min}+(s-{min}) == s;
+
+      [min] + SetToSequenceStr(s-{min})
+  } by method {
+    var a: array<string> := new string[|s|];
+
+    var i := 0;
+    var s' := s;
+    while i < |s|
+      decreases s'
+      invariant |s'| == |s|-i
+      invariant 0 <= i <= |s|
+      invariant (set j | 0 <= j < i :: a[j]) == s-s'
+    {
+      var x :| x in s';
+
+      var a0Seq := a[..];
+
+      a[i] := x;
+
+      assert forall j | 0 <= j < i :: a[j] == a0Seq[j];
+      assert (set j | 0 <= j < i :: a[j]) == s-s';
+
+      var temp := s';
+      s' := s' - {x};
+
+      assert (set j | 0 <= j < i+1 :: a[j]) == (s-temp)+{x};
+      i := i+1;
+    }
+    
+    Sort(a);
+    
+    assert (set j | 0 <= j < i :: a[j]) == s;
+
+    var res := a[..];
+
+    assert res == SetToSequenceStr(s) by {
+      SortedUnique(res, SetToSequenceStr(s), s);
+    }
+
+    return res;
+  }
+
+  predicate method LexRelStr(s1: string, s2: string)
+  {
+    || s1 == []
+    || (s2 != [] && s1[0] < s2[0]) 
+    || (s2 != [] && s1[0] == s2[0] && LexRelStr(s1[1..], s2[1..]))
+  }
+
+lemma {:verify false} LexRelConnex(s1: string, s2: string)
+  ensures LexRelStr(s1, s2) || LexRelStr(s2, s1)
+{ }
+
+lemma {:verify false} LexRelAntisym(s1: string, s2: string)
+  requires LexRelStr(s1, s2)
+  requires LexRelStr(s2, s1)
+  ensures s1 == s2
+{ }
+
+lemma {:verify false} LexRelTransitive(s1: string, s2: string, s3: string)
+  requires LexRelStr(s1, s2)
+  requires LexRelStr(s2, s3)
+  ensures LexRelStr(s1, s3)
+{ }
+
+lemma {:verify false} LexRelIsTotalOrder()
+ensures IsTotalOrder(LexRelStr)
+{
+  forall s1, s2
+  ensures LexRelStr(s1, s2) || LexRelStr(s2, s1)
+  { LexRelConnex(s1, s2); }
+
+  forall s1, s2 | LexRelStr(s1, s2) && LexRelStr(s2, s1)
+  ensures s1 == s2
+  { LexRelAntisym(s1, s2); }
+
+  forall s1, s2, s3 | LexRelStr(s1, s2) && LexRelStr(s2, s3)
+  ensures LexRelStr(s1, s3)
+  { LexRelTransitive(s1, s2, s3); }
+}
+  
+
+/** 
+following definitions taken from http://leino.science/papers/krml275.html
+*/
+
+predicate IsTotalOrder<A(!new)>(R: (A, A) -> bool) {
+  // connexity
+  && (forall a, b :: R(a, b) || R(b, a))
+  // antisymmetry
+  && (forall a, b :: R(a, b) && R(b, a) ==> a == b)
+  // transitivity
+  && (forall a, b, c :: R(a, b) && R(b, c) ==> R(a, c))
+}
+
+lemma ThereIsAMinimumGeneral<A>(R: (A, A) -> bool, s: set<A>)
+  requires s != {}
+  requires IsTotalOrder(R)
+  ensures exists x :: x in s && forall y | y in s :: R(x, y)
+{
+  var x :| x in s;
+  if s == {x} {
+    // obviously, x is the minimum
+    assert x in s;
+    assert forall y | y in s :: x == y;
+  } else {
+    // The minimum in s might be x, or it might be the minimum
+    // in s - {x}. If we knew the minimum of the latter, then
+    // we could compare the two.
+    // Let's start by giving a name to the smaller set:
+    var s' := s - {x};
+    // So, s is the union of s' and {x}:
+    assert s == s' + {x};
+    // The following lemma {:verify false} call establishes that there is a
+    // minimum in s'.
+    ThereIsAMinimumGeneral(R, s');
+    var x' :| x' in s' && forall y | y in s' :: R(x', y);
+
+    var xMin := if R(x, x') then x else x';
+
+    assert xMin in s;
+    forall y | y in s
+    ensures R(xMin, y)
+    {
+      if y == x {
+        if xMin == x {
+
+        }   
+      } else {
+      }
+    }
+  }
+}
+
+lemma ThereIsAMinimum(s: set<string>)
+  requires s != {}
+  ensures exists x :: x in s && forall y | y in s :: LexRelStr(x, y)
+{
+  assert IsTotalOrder(LexRelStr) by {
+    LexRelIsTotalOrder();
+  }
+
+  ThereIsAMinimumGeneral(LexRelStr, s);
+}
 
 }
